Wrote up multisubst

03Debruijn/Multisubst.thy
@@ -2,23 +2,53 @@ theory Multisubst
   imports DebruijnIndices
 begin
 
-inductive tc_pairs :: "ty list \<Rightarrow> expr\<^sub>d list \<Rightarrow> bool" where
-  tcp_nil [simp]: "tc_pairs [] []"
-| tcp_cons [simp]: "[] \<turnstile>\<^sub>d e : t \<Longrightarrow> value\<^sub>d e \<Longrightarrow> tc_pairs \<Gamma> es \<Longrightarrow> tc_pairs (t # \<Gamma>) (e # es)"
+subsection \<open>Multiple substitution\<close>
+
+text \<open>We now want to prove termination. But in order to do that, we need one more tool. Multiple
+substitution replaces every free variable in an expression with a sequence of closed expressions.\<close>
 
 primrec multisubst :: "expr\<^sub>d list \<Rightarrow> expr\<^sub>d \<Rightarrow> expr\<^sub>d" where
   "multisubst [] e = e"
 | "multisubst (e' # es) e = multisubst es (subst\<^sub>d 0 e' e)"
 
-lemma [simp]: "tc_pairs \<Gamma> es \<Longrightarrow> value\<^sub>d e \<Longrightarrow> x \<le> length \<Gamma> \<Longrightarrow> [] \<turnstile>\<^sub>d e : t \<Longrightarrow> 
-  tc_pairs (insert_at x t \<Gamma>) (insert_at x e es)"
-proof (induction \<Gamma> es arbitrary: x rule: tc_pairs.induct)
+lemma multisubst_no_vars [simp]: "[] \<turnstile>\<^sub>d e : t \<Longrightarrow> multisubst es e = e"
+  by (induction es) simp_all
+
+text \<open>Explicitly multiple-substituting over constructors is easy in every case but one. Binders 
+cause problems for a simple compositional definition, because they increment the substitution index
+and \<open>multisubst\<close> only substitutes at 0. We provide a simple solution here and a more precise one, 
+using typechecking side conditions, below.\<close>
+
+lemma multisubst_var [simp]: "lookup vs x = Some v \<Longrightarrow> 
+    (\<And>v es. v \<in> set vs \<Longrightarrow> multisubst es v = v) \<Longrightarrow> multisubst vs (Var\<^sub>d x) = v"
+  by (induction vs x rule: lookup.induct) simp_all
+
+lemma multisubst_const [simp]: "multisubst es (Const\<^sub>d n) = Const\<^sub>d n"
+  by (induction es) simp_all
+
+lemma multisubst_lam_simple [simp]: "\<exists>e'. multisubst es (Lam\<^sub>d t e) = Lam\<^sub>d t e'"
+  by (induction es arbitrary: e) simp_all
+
+lemma multisubst_app [simp]: "multisubst es (App\<^sub>d e\<^sub>1 e\<^sub>2) = App\<^sub>d (multisubst es e\<^sub>1) (multisubst es e\<^sub>2)"
+  by (induction es arbitrary: e\<^sub>1 e\<^sub>2) simp_all
+
+text \<open>Typechecking the sequence of expressions to be multiply-substituted in is simple: they must 
+all be closed values, and they must match the typing context type-for-type. \<close>
+
+inductive tc_expr_context :: "ty list \<Rightarrow> expr\<^sub>d list \<Rightarrow> bool" where
+  tcp_nil [simp]: "tc_expr_context [] []"
+| tcp_cons [simp]: "[] \<turnstile>\<^sub>d e : t \<Longrightarrow> value\<^sub>d e \<Longrightarrow> tc_expr_context \<Gamma> es \<Longrightarrow> 
+    tc_expr_context (t # \<Gamma>) (e # es)"
+
+lemma tc_expr_context_insert [simp]: "tc_expr_context \<Gamma> es \<Longrightarrow> value\<^sub>d e \<Longrightarrow> x \<le> length \<Gamma> \<Longrightarrow> 
+  [] \<turnstile>\<^sub>d e : t \<Longrightarrow> tc_expr_context (insert_at x t \<Gamma>) (insert_at x e es)"
+proof (induction \<Gamma> es arbitrary: x rule: tc_expr_context.induct)
   case (tcp_cons t' e' \<Gamma> es)
   then show ?case by (induction x) simp_all
 qed simp_all
 
-lemma [simp]: "tc_pairs \<Gamma> es \<Longrightarrow> \<Gamma> \<turnstile>\<^sub>d e : t \<Longrightarrow> [] \<turnstile>\<^sub>d multisubst es e : t"
-proof (induction \<Gamma> es arbitrary: e rule: tc_pairs.induct)
+lemma tc_multisubst [simp]: "tc_expr_context \<Gamma> es \<Longrightarrow> \<Gamma> \<turnstile>\<^sub>d e : t \<Longrightarrow> [] \<turnstile>\<^sub>d multisubst es e : t"
+proof (induction \<Gamma> es arbitrary: e rule: tc_expr_context.induct)
   case (tcp_cons e' t' \<Gamma> es)
   moreover hence "insert_at 0 t' \<Gamma> \<turnstile>\<^sub>d e : t" by (induction \<Gamma>) simp_all
   moreover from tcp_cons have "[] \<turnstile>\<^sub>d e' : t'" by simp
@@ -26,47 +56,15 @@ proof (induction \<Gamma> es arbitrary: e rule: tc_pairs.induct)
   ultimately show ?case by simp
 qed simp_all
 
-lemma [simp]: "[] \<turnstile>\<^sub>d e : t \<Longrightarrow> multisubst es e = e"
-  by (induction es) simp_all
-
-lemma multisubst_var [simp]: "lookup vs x = Some v \<Longrightarrow> 
-    (\<And>v es. v \<in> set vs \<Longrightarrow> multisubst es v = v) \<Longrightarrow> multisubst vs (Var\<^sub>d x) = v"
-  by (induction vs x rule: lookup.induct) simp_all
-
-lemma [simp]: "multisubst es (Const\<^sub>d k) = Const\<^sub>d k"
-  by (induction es) simp_all
-
-lemma [simp]: "\<exists>e'. multisubst es (Lam\<^sub>d t e) = Lam\<^sub>d t e'"
-  by (induction es arbitrary: e) simp_all
-
-lemma [simp]: "\<exists>e'. multisubst es (Lam\<^sub>d t e) = Lam\<^sub>d t e' \<and> 
-    (\<forall>e\<^sub>2. (\<forall>ee. subst\<^sub>d 0 ee e\<^sub>2 = e\<^sub>2) \<longrightarrow> subst\<^sub>d 0 e\<^sub>2 e' = multisubst es (subst\<^sub>d 0 e\<^sub>2 e))"
-  by (induction es arbitrary: e) simp_all
-
-lemma [simp]: "tc_pairs \<Gamma> es \<Longrightarrow> insert_at 0 t\<^sub>1 \<Gamma> \<turnstile>\<^sub>d e : t\<^sub>2 \<Longrightarrow> 
+lemma multisubst_lam_complex [simp]: "tc_expr_context \<Gamma> es \<Longrightarrow> insert_at 0 t\<^sub>1 \<Gamma> \<turnstile>\<^sub>d e : t\<^sub>2 \<Longrightarrow> 
   \<exists>e'. multisubst es (Lam\<^sub>d t\<^sub>1 e) = Lam\<^sub>d t\<^sub>1 e' \<and> ([t\<^sub>1] \<turnstile>\<^sub>d e' : t\<^sub>2) \<and>
-    (\<forall>e\<^sub>2. ([] \<turnstile>\<^sub>d e\<^sub>2 : t\<^sub>1) \<longrightarrow> multisubst (insert_at 0 e\<^sub>2 es) e = subst\<^sub>d 0 e\<^sub>2 e')"
-proof (induction \<Gamma> es arbitrary: e rule: tc_pairs.induct)
+    (\<forall>e\<^sub>2. ([] \<turnstile>\<^sub>d e\<^sub>2 : t\<^sub>1) \<longrightarrow> multisubst es (subst\<^sub>d 0 e\<^sub>2 e) = subst\<^sub>d 0 e\<^sub>2 e')"
+proof (induction \<Gamma> es arbitrary: e rule: tc_expr_context.induct)
   case (tcp_cons e' t \<Gamma> es)
   hence "[] \<turnstile>\<^sub>d e' : t" by simp
   hence "\<Gamma> \<turnstile>\<^sub>d e' : t" using tc_postpend by fastforce
   hence "insert_at 0 t\<^sub>1 \<Gamma> \<turnstile>\<^sub>d incr\<^sub>d 0 e' : t" by simp
-  with tcp_cons have "insert_at 0 t\<^sub>1 \<Gamma> \<turnstile>\<^sub>d subst\<^sub>d (Suc 0) (incr\<^sub>d 0 e') e : t\<^sub>2" 
-    by (induction \<Gamma>) simp_all
-  with tcp_cons obtain ee' where E: "([t\<^sub>1] \<turnstile>\<^sub>d ee' : t\<^sub>2) \<and> 
-    multisubst es (Lam\<^sub>d t\<^sub>1 (subst\<^sub>d (Suc 0) (incr\<^sub>d 0 e') e)) = Lam\<^sub>d t\<^sub>1 ee' \<and> 
-      (\<forall>e\<^sub>2. ([] \<turnstile>\<^sub>d e\<^sub>2 : t\<^sub>1) \<longrightarrow> 
-        multisubst (insert_at 0 e\<^sub>2 es) (subst\<^sub>d (Suc 0) (incr\<^sub>d 0 e') e) = subst\<^sub>d 0 e\<^sub>2 ee')" 
-    by fastforce
-  hence "\<And>e\<^sub>2. [] \<turnstile>\<^sub>d e\<^sub>2 : t\<^sub>1 \<Longrightarrow> 
-    multisubst es (subst\<^sub>d 0 e\<^sub>2 (subst\<^sub>d (Suc 0) (incr\<^sub>d 0 e') e)) = subst\<^sub>d 0 e\<^sub>2 ee'" 
-      by (induction es) simp_all
-  hence "\<And>e\<^sub>2. [] \<turnstile>\<^sub>d e\<^sub>2 : t\<^sub>1 \<Longrightarrow> multisubst es (subst\<^sub>d 0 e' (subst\<^sub>d 0 e\<^sub>2 e)) = subst\<^sub>d 0 e\<^sub>2 ee'"
-    by fastforce
-  with E show ?case by simp
+  with tcp_cons show ?case by (cases \<Gamma>) simp_all
 qed simp_all
-
-lemma [simp]: "multisubst es (App\<^sub>d e\<^sub>1 e\<^sub>2) = App\<^sub>d (multisubst es e\<^sub>1) (multisubst es e\<^sub>2)"
-  by (induction es arbitrary: e\<^sub>1 e\<^sub>2) simp_all
 
 end
